Specs to more general

specs/ecdsap256/Spec.DH.fst
@@ -4,30 +4,31 @@ open Lib.IntTypes
 open Lib.ByteSequence
 open Lib.Sequence
 
-open Spec.P256
 open Spec.ECDSA
+
+open Spec.P256
 
 #set-options "--fuel 0 --ifuel 0"
 
 (* Initiator *)
-val ecp256_dh_i: s:lbytes 32 -> tuple3 (lbytes 32) (lbytes 32) uint64
+val ecp256_dh_i: #c: curve -> s:lbytes (getCoordinateLen c) -> tuple3 (lbytes (getCoordinateLen c)) (lbytes (getCoordinateLen c)) uint64
 
-let ecp256_dh_i s =
-  let xN, yN, zN = secret_to_public s in
+let ecp256_dh_i #c s =
+  let xN, yN, zN = secret_to_public #c s in
   if isPointAtInfinity (xN, yN, zN) then
-    nat_to_bytes_be 32 xN, nat_to_bytes_be 32 yN, u64 (pow2 64 - 1)
+    nat_to_bytes_be (getCoordinateLen c) xN, nat_to_bytes_be (getCoordinateLen c) yN, u64 (pow2 64 - 1)
   else
-    nat_to_bytes_be 32 xN, nat_to_bytes_be 32 yN, (u64 0)
+    nat_to_bytes_be (getCoordinateLen c) xN, nat_to_bytes_be (getCoordinateLen c) yN, (u64 0)
 
 
 (* Responder *)
-val ecp256_dh_r: x:lbytes 32 -> y:lbytes 32 -> s:lbytes 32
-  -> tuple3 (lbytes 32) (lbytes 32) uint64
+val ecp256_dh_r: #c: curve -> x:lbytes (getCoordinateLen c) -> y:lbytes (getCoordinateLen c) -> s:lbytes (getCoordinateLen c)
+  -> tuple3 (lbytes (getCoordinateLen c)) (lbytes (getCoordinateLen c)) uint64
 
-let ecp256_dh_r x y s =
+let ecp256_dh_r #c x y s =
   let x_, y_ = nat_from_bytes_be x, nat_from_bytes_be y in
   let pointJacX, pointJacY, pointJacZ = toJacobianCoordinates (x_, y_) in
-  if verifyQValidCurvePointSpec (pointJacX, pointJacY, pointJacZ) then
+  if verifyQValidCurvePointSpec #c (pointJacX, pointJacY, pointJacZ) then
     let xN, yN, zN = scalar_multiplication s (pointJacX, pointJacY, pointJacZ) in
     if isPointAtInfinity (xN, yN, zN) then
       nat_to_bytes_be 32 xN, nat_to_bytes_be 32 yN, u64 (pow2 64 - 1)
